Tv/App.lean
@@ -51,7 +51,7 @@ def handleInput (s : State) (v : View) (di : DisplayInfo) (ev : Term.Event) : IO
       if cmd.startsWith "freq " then
         let cols := (cmd.drop 5).trim.splitOn "," |>.map String.trim
         let prql := (Prql.Query.parse v.prql).freqFull cols |>.render
-        let nav := { NavState.create with keyCols := List.range cols.length }
+        let nav := { NavState.create with keyCols := cols }
         let fv : View := ⟨v.path, prql, s!"freq {String.intercalate "," cols}", nav, .freqV (String.intercalate "," cols), none, [], [], none, 3⟩
         return some { s.push fv with inputMode := .none, inputBuf := "" }
       else if cmd.startsWith "lr " then
